src/Framework/Layer/Operation.v
@@ -12,26 +12,41 @@ Record Operation :=
     exec: forall T, oracle -> state -> prog T -> @Result state T -> Prop;
     weakest_precondition: forall T, prog T -> (T -> state -> Prop) -> (oracle -> state -> Prop);
     weakest_crash_precondition: forall T, prog T -> (state -> Prop) -> (oracle -> state -> Prop);
+    strongest_postcondition: forall T, prog T -> (oracle -> state -> Prop) -> (T -> state -> Prop);
+    strongest_crash_postcondition: forall T, prog T -> (oracle -> state -> Prop) -> (state -> Prop);
+
     wp_complete:
-      forall T (p: prog T) H Q,
-        (forall o s, H o s -> weakest_precondition p Q o s) <->
-        (forall o s, H o s ->
-                (exists s' v, exec o s p (Finished s' v) /\ Q v s'));
+      forall T (p: prog T) P Q,
+        (forall o s, P o s -> weakest_precondition p Q o s) <->
+        (forall o s, P o s -> exists s' v, exec o s p (Finished s' v) /\ Q v s');
     wcp_complete:
-      forall T (p: prog T) H C,
-        (forall o s, H o s -> weakest_crash_precondition p C o s) <->
-        (forall o s, H o s ->
-            (exists s', exec o s p (Crashed s') /\ C s'));
-      exec_deterministic_wrt_oracle :
-        forall o s T (p: prog T) ret1 ret2,
-          exec o s p ret1 ->
-          exec o s p ret2 ->
-          ret1 = ret2;
+      forall T (p: prog T) P C,
+        (forall o s, P o s -> weakest_crash_precondition p C o s) <->
+        (forall o s, P o s -> exists s', exec o s p (Crashed s') /\ C s');
+
+    sp_complete:
+      forall T (p: prog T) P (Q: T -> state -> Prop),
+        (forall t s', strongest_postcondition p P t s' -> Q t s') <->
+        (forall o s s' t, P o s -> exec o s p (Finished s' t) -> Q t s');
+
+    scp_complete:
+      forall T (p: prog T) P (C: state -> Prop),
+        (forall s', strongest_crash_postcondition p P s' -> C s') <->
+        (forall o s s', P o s -> exec o s p (Crashed s') ->  C s');
+    
+    exec_deterministic_wrt_oracle :
+      forall o s T (p: prog T) ret1 ret2,
+        exec o s p ret1 ->
+        exec o s p ret2 ->
+        ret1 = ret2;
   }.
 
 Arguments exec _ {T}.
 Arguments weakest_precondition _ {T}.
 Arguments weakest_crash_precondition _ {T}.
+Arguments strongest_postcondition _ {T}.
+Arguments strongest_crash_postcondition _ {T}.
+
 
 Lemma wp_to_exec:
   forall O T (p: @prog O T) Q o s,
@@ -69,4 +84,71 @@ Proof.
   eapply wcp_complete; intros.
   apply X.
   simpl; eauto.
+Qed.
+
+
+Lemma sp_to_exec:
+  forall O T (p: @prog O T) P t s',
+    strongest_postcondition _ p P t s' -> (exists o s, exec _ o s p (Finished s' t) /\ P o s).
+Proof.
+  intros. edestruct sp_complete; eauto.
+  instantiate (1:= fun t s' => exists (o : oracle O) (s : state O), exec O o s p (Finished s' t) /\ P o s) in H1;
+  simpl in *.
+  eapply H1; intros; eauto.
+Qed.
+
+Lemma exec_to_sp:
+  forall O T (p: @prog O T) (P: _ -> _ -> Prop) o s t s',
+    P o s ->
+    exec _ o s p (Finished s' t) ->
+    strongest_postcondition _ p P t s'.
+Proof.
+  intros. edestruct sp_complete; eauto.
+  eapply H2; eauto.
+Qed.
+
+Lemma scp_to_exec:
+  forall O T (p: @prog O T) P s',
+    strongest_crash_postcondition _ p P s' -> (exists o s, exec _ o s p (Crashed s') /\ P o s).
+Proof.
+  intros. edestruct scp_complete; eauto.
+  instantiate (1:= fun s' => exists (o : oracle O) (s : state O), exec O o s p (Crashed s') /\ P o s) in H1;
+  simpl in *.
+  eapply H1; intros; eauto.
+Qed.
+
+Lemma exec_to_scp:
+  forall O T (p: @prog O T) (P: _ -> _ -> Prop) o s s',
+    P o s ->
+    exec _ o s p (Crashed s') ->
+    strongest_crash_postcondition _ p P s'.
+Proof.
+  intros. edestruct scp_complete; eauto.
+  eapply H2; eauto.
+Qed.
+
+
+
+Lemma sp_post:
+  forall O T (p: @prog O T) (P: oracle _ -> state _ -> Prop) o s s' t,
+    P o s ->
+    exec _ o s p (Finished s' t) ->
+    strongest_postcondition _ p P t s'.
+Proof.
+  intros.
+  edestruct sp_complete.
+  eapply H1; eauto.
+Qed.
+
+Lemma sp_strongest:
+  forall O T (p: @prog O T) (P: oracle _ -> state _ -> Prop) (Q: T -> state _ -> Prop),
+    (forall o s s' t,
+       P o s -> 
+       exec _ o s p (Finished s' t) ->
+       Q t s') ->
+    (forall t s', strongest_postcondition _ p P t s' -> Q t s').
+Proof.
+  intros.
+  edestruct sp_complete.
+  eapply H2; eauto.  
 Qed.
